src/Eqvivalence/BsFs/NewEraseNames.v
@@ -1,0 +1,1388 @@
+From CoreErlang.Eqvivalence Require Export Basics.
+
+Import BigStep.
+
+(** CONTENT:
+* MEASURE_VALUE (DEFINITIONS)
+  - MeasureValue_Helpers
+    + measure_val_list
+    + measure_val_map
+    + measure_val_env
+  - MeasureValue_Main
+    + measure_val
+* REMOVE_FROM_ENVIRONMENT (DEFINITIONS, LEMMAS)
+  - RemoveFromEnvironment (DEFINITIONS)
+    + rem_keys
+    + rem_fids
+    + rem_vars
+    + rem_ext
+    + rem_ext_vars
+  - RemoveFromEnvironment_Empty (LEMMAS)
+    + rem_keys_empty
+    + rem_fids_empty
+    + rem_vars_empty
+    + rem_ext_empty
+    + rem_ext_vars_empty_ext
+    + rem_ext_vars_empty_vars
+    + rem_ext_vars_empty
+  - RemoveFromEnvironment_Append (LEMMAS)
+    + rem_keys_app
+    + rem_ext_vars_app
+* ADD_TO_ERASER (TYPE, DEFINITIONS)
+  - AddToEraser_Helpers (DEFINITIONS)
+    + convert_lit
+    + vars_of_pattern_list
+    + sum_eqb
+  - AddToEraser_Types (TYPE)
+    + NameSub
+    + Eraser
+    + σ0
+  - AddToEraser (DEFINITIONS)
+    + add_name
+    + add_names
+    + add_keys
+    + add_fids
+    + add_vars
+    + add_ext
+    + add_ext_vars
+    + add_expext
+    + add_expext_vars
+    + add_pats
+    + add_env
+    + from_env
+  - AddToEraser_Empty (LEMMAS)
+    + add_keys_empty
+    + add_fids_empty
+    + add_vars_empty
+    + add_ext_empty
+    + add_ext_vars_empty_ext
+    + add_ext_vars_empty_vars
+    + add_ext_vars_empty
+  - AddToEraser_Append (LEMMAS)
+    + add_keys_app
+    + add_ext_vars_app
+* ERASE_NAMES (DEFINITIONS)
+  - EraseNames_Bigs
+    + erase_pat
+    + erase_exp
+    + erase_val
+    + erase_val'
+  - EraseNames_Smalls
+    + erase_names
+    + convert_class
+    + erase_exc
+    + erase_result
+  - EraseNames_Axioms
+    + erase_val_fuel
+  - EraseNames_Lemmas
+    + erase_val_fuel_list
+    + erase_val_fuel_fun
+    + erase_val_fuel_map
+  - EraseNames_Tactics
+    + mvr (Measure Value Reduction)
+*)
+
+
+
+
+
+
+
+
+
+
+
+
+(*
+////////////////////////////////////////////////////////////////////////////////
+//// CHAPTER: MEASURE_VALUE ////////////////////////////////////////////////////
+////////////////////////////////////////////////////////////////////////////////
+*)
+
+
+
+
+
+
+Section MeasureValue_Helpers.
+
+
+
+  Definition measure_val_list
+      (measure : Value -> nat)
+      (vl : list Value)
+      : nat 
+      :=
+    list_sum (map measure vl).
+
+
+
+  Definition measure_val_map
+      (measure : Value -> nat)
+      (vll : list (Value * Value))
+      : nat
+      :=
+    list_sum (map (fun '(x, y) => (measure x) + (measure y)) vll).
+
+
+
+  Definition measure_val_env
+      (measure : Value -> nat)
+      (Γ : Environment)
+      : nat
+      :=
+    list_sum (map (measure ∘ snd) Γ).
+
+
+
+End MeasureValue_Helpers.
+
+
+
+
+
+
+
+
+
+Section MeasureValue_Main.
+
+
+
+  Fixpoint measure_val
+      (v : Value) 
+      : nat
+      :=
+    match v with
+
+    | VNil => 1
+    | VLit l => 1
+
+    | VCons v1 v2 => 1
+      + measure_val v1
+      + measure_val v2
+
+    | VTuple vl => 1
+      + measure_val_list measure_val vl
+
+    | VMap vll => 1
+      + measure_val_map measure_val vll
+
+    | VClos Γ ext _ _ e => 2
+      + measure_val_env measure_val Γ
+
+    end.
+
+
+
+End MeasureValue_Main.
+
+
+
+
+
+
+
+
+
+
+
+
+(*
+////////////////////////////////////////////////////////////////////////////////
+//// CHAPTER: REMOVE_FROM_ENVIRONMENT //////////////////////////////////////////
+////////////////////////////////////////////////////////////////////////////////
+*)
+
+
+
+
+
+
+Section RemoveFromEnvironment.
+
+
+
+  Definition rem_keys
+      (keys : list (Var + FunctionIdentifier))
+      (Γ : Environment)
+      : Environment
+      :=
+    filter
+      (fun '(k, v) =>
+        negb (existsb
+          (fun x => (var_funid_eqb x k))
+          keys))
+      Γ.
+
+
+
+  Definition rem_fids
+      (fids : list FunctionIdentifier)
+      (Γ : Environment)
+      : Environment
+      :=
+    rem_keys (map inr fids) Γ.
+
+
+
+  Definition rem_vars
+      (vars : list Var)
+      (Γ : Environment)
+      : Environment
+      :=
+    rem_keys (map inl vars) Γ.
+
+
+
+  Definition rem_ext
+      (ext : list (nat * FunctionIdentifier * FunctionExpression))
+      (Γ : Environment)
+      : Environment
+      :=
+    rem_fids (map (snd ∘ fst) ext) Γ.
+
+
+
+  Definition rem_ext_vars
+      (ext : list (nat * FunctionIdentifier * FunctionExpression))
+      (vars : list Var)
+      (Γ : Environment)
+      : Environment
+      :=
+    rem_ext ext (rem_vars vars Γ).
+
+
+
+End RemoveFromEnvironment.
+
+
+
+
+
+
+
+
+
+Section RemoveFromEnvironment_Empty.
+
+
+
+  Lemma rem_keys_empty :
+    forall Γ,
+      rem_keys [] Γ = Γ.
+  Proof.
+    (* #1 Induction on Environment: induction + simpl*)
+    ind - Γ as [| [k v] Γ IH] :> smp.
+    (* #2 Rewrite by Induction: rewrite *)
+    bwr - IH.
+  Qed.
+
+
+
+  Lemma rem_fids_empty :
+    forall Γ,
+      rem_fids [] Γ = Γ.
+  Proof.
+    app - rem_keys_empty.
+  Qed.
+
+
+
+  Lemma rem_vars_empty :
+    forall Γ,
+      rem_vars [] Γ = Γ.
+  Proof.
+    app - rem_keys_empty.
+  Qed.
+
+
+
+  Lemma rem_ext_empty :
+    forall Γ,
+      rem_ext [] Γ = Γ.
+  Proof.
+    app - rem_keys_empty.
+  Qed.
+
+
+
+  Lemma rem_ext_vars_empty_ext :
+    forall vars Γ,
+      rem_ext_vars [] vars Γ = rem_vars vars Γ.
+  Proof.
+    itr.
+    ufl - rem_ext_vars.
+    bwr - rem_ext_empty.
+  Qed.
+
+
+
+  Lemma rem_ext_vars_empty_vars :
+    forall ext Γ,
+      rem_ext_vars ext [] Γ = rem_ext ext Γ.
+  Proof.
+    itr.
+    ufl - rem_ext_vars.
+    bwr - rem_vars_empty.
+  Qed.
+
+
+
+  Lemma rem_ext_vars_empty :
+    forall Γ,
+      rem_ext_vars [] [] Γ = Γ.
+  Proof.
+    itr.
+    ufl - rem_ext_vars.
+    bwr - rem_ext_empty
+          rem_vars_empty.
+  Qed.
+
+
+
+End RemoveFromEnvironment_Empty.
+
+
+
+
+
+
+
+
+
+Section RemoveFromEnvironment_Append.
+
+
+
+  Lemma rem_keys_app :
+    forall keys1 keys2 Γ,
+      rem_keys (keys1 ++ keys2) Γ
+    = rem_keys keys1 (rem_keys keys2 Γ).
+  Proof.
+    itr.
+    ind - Γ as [| [k v] Γ IHΓ]: smp.
+    ufl - rem_keys in *.
+    smp *.
+    rwr - existsb_app.
+    rwr - negb_orb.
+    des > ((negb (existsb (fun x => var_funid_eqb x k) keys1))) as Hkeys1;
+    des > ((negb (existsb (fun x => var_funid_eqb x k) keys2))) as Hkeys2;
+    smp.
+    * rwr - Hkeys1.
+      bwr - IHΓ.
+    * bwr - IHΓ.
+    * rwr - Hkeys1.
+      bwr - IHΓ.
+    * bwr - IHΓ.
+  Qed.
+
+
+
+  Lemma rem_ext_vars_app :
+    forall ext vars Γ,
+      rem_keys ((map (inr ∘ snd ∘ fst) ext) ++ (map inl vars)) Γ
+    = rem_ext_vars ext vars Γ.
+  Proof.
+    itr.
+    rwr - rem_keys_app.
+    ufl - rem_ext_vars
+          rem_ext
+          rem_vars
+          rem_fids.
+    bwr - map_map.
+  Qed.
+
+
+
+End RemoveFromEnvironment_Append.
+
+
+
+
+
+
+
+
+
+
+
+
+(*
+////////////////////////////////////////////////////////////////////////////////
+//// CHAPTER: ADD_TO_ERASER ////////////////////////////////////////////////////
+////////////////////////////////////////////////////////////////////////////////
+*)
+
+
+
+
+
+
+Section AddToEraser_Helpers.
+
+
+
+  Definition convert_lit
+      (lit : Literal)
+      : Lit
+      :=
+    match lit with
+     | Atom s => s
+     | Integer x => x
+    end.
+
+
+
+  Definition convert_class
+      (class : ExceptionClass)
+      : ExcClass
+      :=
+    match class with
+    | Error =>  CoreErlang.Syntax.Error
+    | Throw =>  CoreErlang.Syntax.Throw
+    | Exit =>   CoreErlang.Syntax.Exit
+    end.
+
+
+
+  Definition vars_of_pattern_list
+      (pl : list Pattern)
+      : list Var
+      :=
+    fold_right
+      (fun x acc => variable_occurances x ++ acc)
+      nil
+      pl.
+
+
+
+  Definition sum_eqb
+      {A B : Type}
+      (eqbA : A -> A -> bool)
+      (eqbB : B -> B -> bool)
+      (a b : A + B)
+      : bool
+      :=
+    match a, b with
+    | inl a', inl b' => eqbA a' b'
+    | inr a', inr b' => eqbB a' b'
+    | _, _ => false
+    end.
+
+
+
+End AddToEraser_Helpers.
+
+
+
+
+
+
+
+
+
+Section AddToEraser_Types.
+
+
+
+  Definition NameSub
+      {T}
+      {dec : T -> T -> bool}
+      :=
+    T -> nat.
+
+
+
+  Definition Eraser
+      :=
+    @NameSub
+      (Var + FunctionIdentifier)
+      (sum_eqb eqb (prod_eqb eqb Nat.eqb)).
+
+
+
+  Definition σ0 : Eraser := (fun _ => 0).
+
+
+
+End AddToEraser_Types.
+
+
+
+
+
+
+
+
+
+Section AddToEraser.
+
+
+
+  Definition add_name
+      {T dec}
+      (name : T)
+      (σ : @NameSub _ dec)
+      :=
+    fun x =>
+      if dec x name
+      then 0
+      else S (σ x).
+
+
+
+  Definition add_names
+      {T}
+      {dec : T -> T -> bool}
+      (names : list T)
+      (σ : NameSub)
+      : NameSub
+      :=
+    fold_right
+      (@add_name _ dec)
+      σ
+      names.
+
+
+
+
+
+
+  Definition add_keys
+      (keys : list (Var + FunctionIdentifier))
+      (σ : Eraser)
+      : Eraser
+      :=
+    add_names keys σ.
+
+
+
+  Definition add_fids
+      (fids : list FunctionIdentifier)
+      (σ : Eraser)
+      : Eraser
+      :=
+    add_keys (map inr fids) σ.
+
+
+
+  Definition add_vars
+      (vars : list Var)
+      (σ : Eraser)
+      : Eraser
+      :=
+    add_keys (map inl vars) σ.
+
+
+
+  Definition add_ext
+      (ext : list (nat * FunctionIdentifier * FunctionExpression))
+      (σ : Eraser)
+      : Eraser
+      :=
+    add_fids (map (snd ∘ fst) ext) σ.
+
+
+
+  Definition add_ext_vars
+      (ext : list (nat * FunctionIdentifier * FunctionExpression))
+      (vars : list Var)
+      (σ : Eraser)
+      : Eraser
+      :=
+    add_ext ext (add_vars vars σ).
+
+
+
+  Definition add_expext
+      (ext : list (FunctionIdentifier * FunctionExpression))
+      (σ : Eraser)
+      : Eraser
+      :=
+    add_fids (map fst ext) σ.
+
+
+
+  Definition add_expext_vars
+      (ext : list (FunctionIdentifier * FunctionExpression))
+      (vars : list Var)
+      (σ : Eraser)
+      : Eraser
+      :=
+    add_expext ext (add_vars vars σ).
+
+
+
+  Definition add_pats
+      (pats : list Pattern)
+      (σ : Eraser)
+      : Eraser
+      :=
+    add_vars (vars_of_pattern_list pats) σ.
+
+
+
+  Definition add_env
+      (Γ : Environment)
+      (σ : Eraser)
+      : Eraser
+      :=
+    add_keys (map fst Γ) σ.
+
+
+
+  Definition from_env
+      (Γ : Environment)
+      : Eraser
+      :=
+    add_env Γ σ0.
+
+
+
+End AddToEraser.
+
+
+
+
+
+
+
+
+
+Section AddToEraser_Empty.
+
+
+
+  Lemma add_keys_empty :
+    forall σ,
+      add_keys [] σ = σ.
+  Proof.
+    trv.
+  Qed.
+
+
+
+  Lemma add_fids_empty :
+    forall σ,
+      add_fids [] σ = σ.
+  Proof.
+    trv.
+  Qed.
+
+
+
+  Lemma add_vars_empty :
+    forall σ,
+      add_vars [] σ = σ.
+  Proof.
+    trv.
+  Qed.
+
+
+
+  Lemma add_ext_empty :
+    forall σ,
+      add_ext [] σ = σ.
+  Proof.
+    app - add_keys_empty.
+  Qed.
+
+
+
+  Lemma add_ext_vars_empty_ext :
+    forall vars σ,
+      add_ext_vars [] vars σ = add_vars vars σ.
+  Proof.
+    itr.
+    ufl - add_ext_vars.
+    app - add_ext_empty.
+  Qed.
+
+
+
+  Lemma add_ext_vars_empty_vars :
+    forall ext σ,
+      add_ext_vars ext [] σ = add_ext ext σ.
+  Proof.
+    itr.
+    ufl - add_ext_vars.
+    app - add_vars_empty.
+  Qed.
+
+
+
+  Lemma add_ext_vars_empty :
+    forall σ,
+      add_ext_vars [] [] σ = σ.
+  Proof.
+    trv.
+  Qed.
+
+
+
+End AddToEraser_Empty.
+
+
+
+
+
+
+
+
+
+Section AddToEraser_Append.
+
+
+
+  Lemma add_keys_app :
+    forall keys1 keys2 σ,
+      add_keys (keys1 ++ keys2) σ
+    = add_keys keys1 (add_keys keys2 σ).
+  Proof.
+    itr.
+    ufl - add_keys.
+    unfold add_names.
+    bwr - foldr_app.
+  Qed.
+
+
+
+  Lemma add_ext_vars_app :
+    forall ext vars σ,
+      add_keys ((map (inr ∘ snd ∘ fst) ext) ++ (map inl vars)) σ
+    = add_ext_vars ext vars σ.
+  Proof.
+    itr.
+    rwr - add_keys_app.
+    ufl - add_ext_vars
+          add_ext
+          add_vars
+          add_fids.
+    bwr - map_map.
+  Qed.
+
+
+
+End AddToEraser_Append.
+
+
+
+
+
+
+
+
+
+
+
+
+(*
+////////////////////////////////////////////////////////////////////////////////
+//// CHAPTER: ERASE_NAMES //////////////////////////////////////////////////////
+////////////////////////////////////////////////////////////////////////////////
+*)
+
+
+
+Section EraseNames_Bigs.
+
+
+
+  Fixpoint erase_pat
+      (p : Pattern)
+      : Pat
+      :=
+    match p with
+
+    | PNil =>
+      Syntax.PNil
+
+    | PVar _ =>
+      Syntax.PVar
+
+    | PLit lit =>
+      Syntax.PLit
+        (convert_lit lit)
+
+    | PCons p1 p2 =>
+      Syntax.PCons
+        (erase_pat p1)
+        (erase_pat p2)
+
+    | PTuple pl =>
+      Syntax.PTuple
+        (map erase_pat pl)
+
+    | PMap pll =>
+      Syntax.PMap
+        (map
+          (prod_map
+            erase_pat
+            erase_pat)
+          pll)
+
+    end.
+
+
+
+
+
+
+  Fixpoint erase_exp
+      (σ : NameSub)
+      (e : Expression)
+      : Exp
+      :=
+    match e with
+
+    | ENil =>
+      ˝Syntax.VNil
+
+    | ELit lit =>
+      ˝Syntax.VLit
+        (convert_lit lit)
+
+    | ECons e1 e2 =>
+      Syntax.ECons
+        (erase_exp σ e1)
+        (erase_exp σ e2)
+
+    | ESeq e1 e2 =>
+      Syntax.ESeq
+        (erase_exp σ e1)
+        (erase_exp σ e2)
+
+    | EValues el =>
+      Syntax.EValues
+        (map (erase_exp σ) el)
+
+    | ETuple el =>
+      Syntax.ETuple
+        (map (erase_exp σ) el)
+
+    | EPrimOp s el =>
+      Syntax.EPrimOp
+        s
+        (map (erase_exp σ) el)
+
+    | EApp e el =>
+      Syntax.EApp
+        (erase_exp σ e)
+        (map (erase_exp σ) el)
+
+    | ECall e1 e2 el =>
+      Syntax.ECall
+        (erase_exp σ e1)
+        (erase_exp σ e2)
+        (map (erase_exp σ) el)
+
+    | EMap ell =>
+      Syntax.EMap
+        (map
+          (prod_map
+            (erase_exp σ)
+            (erase_exp σ))
+          ell)
+
+    | EFun vars e =>
+      Syntax.EFun
+        (length vars)
+        (erase_exp (add_vars vars σ) e)
+
+    | ELet vars e1 e2 =>
+      Syntax.ELet
+        (length vars)
+        (erase_exp σ e1)
+        (erase_exp (add_vars vars σ) e2)
+
+    | ETry e1 vars1 e2 vars2 e3 =>
+      Syntax.ETry
+        (erase_exp σ e1)
+        (length vars1)
+        (erase_exp (add_vars vars1 σ) e2)
+        (length vars2)
+        (erase_exp (add_vars vars2 σ) e3)
+
+    | ELetRec ext e =>
+      Syntax.ELetRec
+        (map
+          (fun '(_, (vars, body)) =>
+            (length vars,
+            erase_exp (add_expext_vars ext vars σ) body))
+          ext)
+        (erase_exp (add_expext ext σ) e)
+
+    | ECase e case =>
+      Syntax.ECase
+        (erase_exp σ e)
+        (map 
+          (fun '(pats, e1, e2) =>
+            ((map erase_pat pats),
+            erase_exp (add_pats pats σ) e1,
+            erase_exp (add_pats pats σ) e2))
+          case)
+
+    | EVar var =>
+      ˝Syntax.VVar
+        (σ (inl var))
+
+    | EFunId fid =>
+      ˝Syntax.VFunId
+        ((σ (inr fid)), snd fid)
+
+    end.
+
+
+
+
+
+
+  Fixpoint erase_val
+      (n : nat)
+      (v : Value)
+      : Val
+      :=
+
+    let
+      erase_subst
+          (n : nat)
+          (shift : nat)
+          (σ : NameSub)
+          (vl : list Value)
+          (e : Expression)
+          : Exp
+          :=
+        (erase_exp σ e)
+        .[upn shift
+          (list_subst (map (fun v => erase_val n v) vl) idsubst)]
+    in
+
+    let
+      erase_body
+          (n : nat)
+          (Γ : Environment)
+          (ext : list (nat * FunctionIdentifier * FunctionExpression))
+          (vars : list Var)
+          (e : Expression)
+          : Exp
+          :=
+        erase_subst
+          n
+          (length ext + length vars)
+          (add_ext_vars ext vars (from_env (rem_ext_vars ext vars Γ)))
+          (map snd (rem_ext_vars ext vars Γ))
+          e
+        (* Refactor BigStep EFun/Letrec: Γ -> (rem_ext_vars ext vars Γ)  *)
+    in
+
+    let
+      erase_clositem
+          (n : nat)
+          (Γ : Environment)
+          (ext : list (nat * FunctionIdentifier * FunctionExpression))
+          (ci : nat * FunctionIdentifier * FunctionExpression)
+          : nat * nat * Exp
+          :=
+        match ci with
+        | (id, fid, (vars, e)) =>
+          (id, length vars, erase_body n Γ ext vars e)
+        end
+    in
+
+    let
+      erase_ext
+          (n : nat)
+          (Γ : Environment)
+          (ext : list (nat * FunctionIdentifier * FunctionExpression))
+          : list (nat * nat * Exp)
+          :=
+        map (erase_clositem n Γ ext) ext
+    in
+
+    match n with
+    | 0 => Syntax.VNil
+    | S n' =>
+
+      match v with
+
+      | VNil =>
+        Syntax.VNil
+
+      | VLit lit =>
+        Syntax.VLit
+          (convert_lit lit)
+
+      | VCons v1 v2 =>
+        Syntax.VCons
+          (erase_val n' v1)
+          (erase_val n' v2)
+
+      | VTuple vl =>
+        Syntax.VTuple
+          (map (fun v => erase_val n' v) vl)
+
+      | VMap vll =>
+        Syntax.VMap
+          (map
+            (fun '(v1, v2) => (erase_val n' v1, erase_val n' v2))
+            vll)
+
+      | VClos Γ ext _ vars e =>
+        Syntax.VClos
+          (erase_ext n' Γ ext)
+          0
+          (length vars)
+          (erase_body n' Γ ext vars e)
+
+      end
+    end.
+
+
+
+
+
+
+  Definition erase_val'
+      (v : Value)
+      : Val
+      :=
+
+    let
+      erase_subst
+          (shift : nat)
+          (σ : NameSub)
+          (vl : list Value)
+          (e : Expression)
+          : Exp
+          :=
+        (erase_exp σ e)
+        .[upn shift
+          (list_subst (map (fun v => erase_val (measure_val v) v) vl) idsubst)]
+    in
+
+    let
+      erase_body
+          (Γ : Environment)
+          (ext : list (nat * FunctionIdentifier * FunctionExpression))
+          (vars : list Var)
+          (e : Expression)
+          : Exp
+          :=
+        erase_subst
+          (length ext + length vars)
+          (add_ext_vars ext vars (from_env (rem_ext_vars ext vars Γ)))
+          (map snd (rem_ext_vars ext vars Γ))
+          e
+        (* Refactor BigStep EFun/Letrec: Γ -> (rem_ext_vars ext vars Γ)  *)
+    in
+
+    let
+      erase_clositem
+          (Γ : Environment)
+          (ext : list (nat * FunctionIdentifier * FunctionExpression))
+          (ci : nat * FunctionIdentifier * FunctionExpression)
+          : nat * nat * Exp
+          :=
+        match ci with
+        | (id, fid, (vars, e)) =>
+          (id, length vars, erase_body Γ ext vars e)
+        end
+    in
+
+    let
+      erase_ext
+          (Γ : Environment)
+          (ext : list (nat * FunctionIdentifier * FunctionExpression))
+          : list (nat * nat * Exp)
+          :=
+        map (erase_clositem Γ ext) ext
+    in
+
+    match v with
+
+    | VNil =>
+      Syntax.VNil
+
+    | VLit lit =>
+      Syntax.VLit
+        (convert_lit lit)
+
+    | VCons v1 v2 =>
+      Syntax.VCons
+        (erase_val (measure_val v1) v1)
+        (erase_val (measure_val v2) v2)
+
+    | VTuple vl =>
+      Syntax.VTuple
+        (map (fun v => erase_val (measure_val v) v) vl)
+
+    | VMap vll =>
+      Syntax.VMap
+        (map
+          (fun '(v1, v2) =>
+            (erase_val (measure_val v1) v1,
+             erase_val (measure_val v2) v2))
+          vll)
+
+    | VClos Γ ext _ vars e =>
+      Syntax.VClos
+        (erase_ext Γ ext)
+        0
+        (length vars)
+        (erase_body Γ ext vars e)
+
+    end.
+
+
+
+End EraseNames_Bigs.
+
+
+
+
+
+
+
+
+
+Section EraseNames_Smalls.
+
+
+
+  Definition erase_names
+      (Γ : Environment)
+      (e : Expression)
+      : Exp
+      :=
+    (erase_exp (from_env Γ) e)
+    .[list_subst
+      (map erase_val' (map snd Γ))
+      idsubst].
+
+
+
+  Definition erase_valseq
+      (vs : ValueSequence)
+      : ValSeq
+      :=
+    map erase_val' vs.
+
+
+
+  Definition erase_exc
+      (exc : Exception)
+      : CoreErlang.Syntax.Exception
+      :=
+    match exc with
+    | (class, v1, v2) =>
+      (convert_class class, erase_val' v1, erase_val' v2)
+    end.
+
+
+
+  Definition erase_result
+      (result : (ValueSequence + Exception))
+      : Redex
+      :=
+    match result with
+    | inl vs =>   RValSeq (erase_valseq vs)
+    | inr exc =>  RExc (erase_exc exc)
+    end.
+
+
+
+End EraseNames_Smalls.
+
+
+
+
+
+
+
+
+
+Section EraseNames_Notations.
+
+
+(* 
+Notation "δₚ( p )" := (erase_pat p)
+  (p at level 200, format "δₚ( p )" ).
+Notation "δₑ( e / σ )" := (erase_exp σ e)
+  (e at level 200, σ at level 200, format "δₑ( e / σ )" ).
+Notation "δₑ( e ) .[ Γ ]" := (erase_names Γ e)
+  (e at level 200, Γ at level 200, format "δₑ( e ) .[ Γ ]" ).
+
+Lemma tmp : forall p p', erase_pat p = p'. Proof. Admitted.
+Lemma tmp2 : forall σ e e', erase_exp σ e = e'. Proof. Admitted.
+Lemma tmp3 : forall Γ e e', erase_names Γ e = e'. Proof. Admitted.
+
+Notation "'δₑ" := erase_exp.
+Notation "`δᵥ" := erase_val.
+Notation "'δᵥ" := erase_val'.
+Notation "δₑ e .[ Γ ]" := (erase_names Γ e) 
+  (at level 2, Γ at level 200, left associativity,
+   format "δₑ e .[ Γ ]" ).
+
+
+
+(* Example usage of the notation *)
+Lemma example_lemma2 : forall e env, δₑ e .[ Γ ] = δₑ e .[ Γ ] .
+Proof
+  intros.
+  reflexivity.
+Qed. *)
+
+
+
+End EraseNames_Notations.
+
+
+
+
+
+
+
+
+
+Section EraseNames_Axioms.
+
+
+
+  Axiom erase_val_fuel :
+    forall v n,
+      erase_val n v = erase_val' v.
+
+
+
+End EraseNames_Axioms.
+
+
+
+
+
+
+
+
+
+Section EraseNames_Lemmas.
+
+
+
+  Lemma erase_val_fuel_list :
+    forall vl n,
+      map (fun v => erase_val n v) vl
+    = map (fun v => erase_val' v) vl.
+  Proof.
+    itr.
+    ind - vl as [| v vl IHvl]: smp.
+    smp.
+    feq.
+    * app - erase_val_fuel.
+    * exa - IHvl.
+  Qed.
+
+
+
+  Lemma erase_val_fuel_list_measure :
+    forall vl,
+      map (fun v => erase_val (measure_val v) v) vl
+    = map (fun v => erase_val' v) vl.
+  Proof.
+    itr.
+    ind - vl as [| v vl IHvl]: smp.
+    smp.
+    feq.
+    * app - erase_val_fuel.
+    * exa - IHvl.
+  Qed.
+
+
+
+  Lemma erase_val_fuel_fun :
+    forall vl n,
+      map (fun v => erase_val n v) vl
+    = map erase_val' vl.
+  Proof.
+    itr.
+    rwr - erase_val_fuel_list.
+    trv.
+  Qed.
+
+
+
+  Lemma erase_val_fuel_fun_measure :
+    forall vl,
+      map (fun v => erase_val (measure_val v) v) vl
+    = map erase_val' vl.
+  Proof.
+    itr.
+    rwr - erase_val_fuel_list_measure.
+    trv.
+  Qed.
+
+
+
+  Lemma erase_val_fuel_map :
+    forall vll n,
+      map (fun '(v1, v2) => (erase_val n v1, erase_val n v2)) vll
+    = map (fun '(v1, v2) => (erase_val' v1, erase_val' v2)) vll.
+  Proof.
+    itr.
+    ind - vll as [| [v1 v2] vll IHvl]: smp.
+    smp.
+    feq.
+    * feq.
+      - app - erase_val_fuel.
+      - app - erase_val_fuel.
+    * exa - IHvl.
+  Qed.
+
+
+
+  Lemma erase_val_fuel_map_measure :
+    forall vll,
+      map
+        (fun '(v1, v2) =>
+          (erase_val (measure_val v1) v1, erase_val (measure_val v2) v2))
+        vll
+    = map (fun '(v1, v2) => (erase_val' v1, erase_val' v2)) vll.
+  Proof.
+    itr.
+    ind - vll as [| [v1 v2] vll IHvl]: smp.
+    smp.
+    feq.
+    * feq.
+      - app - erase_val_fuel.
+      - app - erase_val_fuel.
+    * exa - IHvl.
+  Qed.
+
+
+
+End EraseNames_Lemmas.
+
+
+
+
+
+
+
+
+
+(* Section EraseNames_Tactics. *)
+
+
+
+  Ltac mvr :=
+    try (rewrite erase_val_fuel in *);
+    try (rewrite erase_val_fuel_list in *);
+    try (rewrite erase_val_fuel_list_measure in *);
+    try (rewrite erase_val_fuel_fun in *);
+    try (rewrite erase_val_fuel_fun_measure in *);
+    try (rewrite erase_val_fuel_map in *);
+    try (rewrite erase_val_fuel_map_measure in *).
+
+
+
+(* End EraseNames_Tactics. *)
